AstSubsetPredicates.dfy
@@ -1,0 +1,72 @@
+include "BoogieLang.dfy"
+
+module AstSubsetPredicates
+{
+  import opened BoogieLang
+  import opened Wrappers
+
+  predicate NoLoops(c: Cmd)
+  {
+    match c
+    case SimpleCmd(_) => true
+    case Break(optLbl) => true
+    case Seq(c1, c2) => NoLoops(c1) && NoLoops(c2)
+    case Loop(_,_) => false
+    case Scope(_, varDecls, body) => NoLoops(body)
+    case If(_, thn, els) => NoLoops(thn) && NoLoops(els)
+  }
+
+  predicate NoIfCond(c: Cmd)
+  {
+    match c
+    case SimpleCmd(_) => true
+    case Break(optLbl) => true
+    case Seq(c1, c2) => NoIfCond(c1) && NoIfCond(c2)
+    case Loop(_, body) => NoIfCond(body)
+    case Scope(_, varDecls, body) => NoIfCond(body)
+    case If(optCond, thn, els) => 
+      && optCond == None 
+      && NoIfCond(thn)
+      && NoIfCond(els)
+  }
+
+  predicate NoLoopsNoIfCond(c: Cmd)
+  {
+    && NoLoops(c) 
+    && NoIfCond(c)
+  }
+
+  predicate NoScopedVars(c: Cmd)
+  {
+    match c
+    case SimpleCmd(_) => true
+    case Break(optLbl) => true
+    case Seq(thn, els) => 
+      && NoScopedVars(thn) 
+      && NoScopedVars(els)
+    case Loop(_,_) => false
+    case Scope(_, varDecls, body) => 
+      && varDecls == [] 
+      && NoScopedVars(body)
+    case If(_, thn, els) => NoScopedVars(thn) && NoScopedVars(els)
+  }
+
+  predicate NoLoopsNoIfCondNoScopedVars(c: Cmd)
+  {
+    && NoLoops(c) 
+    && NoIfCond(c)
+    && NoScopedVars(c)
+  }
+
+
+  predicate NoBreaksScopedVarsLoops(c: Cmd)
+  {
+    match c
+    case SimpleCmd(_) => true
+    case Break(optLbl) => false
+    case Seq(c1, c2) => NoBreaksScopedVarsLoops(c1) && NoBreaksScopedVarsLoops(c2)
+    case Loop(_,_) => false
+    case Scope(_, varDecls, body) => varDecls == [] && NoBreaksScopedVarsLoops(body)
+    case If(_, thn, els) => NoBreaksScopedVarsLoops(thn) && NoBreaksScopedVarsLoops(els)
+  }
+}
